## Question
Given a dataset for a binary classification problem, you've decided to use logistic regression with regularization to prevent overfitting. Your logistic regression model uses a sigmoid function $\sigma(z) = \frac{1}{1 + e^{-z}}$ for predictions, where $z = w_0 + w_1x_1 + w_2x_2 + ... + w_nx_n$ and L2 regularization for its cost function. The regularized cost function $J(w)$ for logistic regression is given as:

$$J(w) = -\frac{1}{m}\sum_{i=1}^{m}[y^{(i)}\log(\sigma(z^{(i)})) + (1-y^{(i)})\log(1-\sigma(z^{(i)}))] + \frac{\lambda}{2m}\sum_{j=1}^{n}w_j^2$$

where $m$ is the number of training examples, $n$ is the number of features, $y^{(i)}$ is the actual label for the $i$-th training example, $w$ are the parameters (weights), $\lambda$ is the regularization parameter, and $\sigma(z^{(i)})$ is the prediction for the $i$-th training example.

To train this logistic regression model using gradient descent, you will need to compute the gradient of $J(w)$ with respect to each weight $w_j$. Which of the following correctly represents the derivative of $J(w)$ with respect to $w_j$ (for $j \ge 1$)?

1. $\frac{\partial J}{\partial w_j} = \frac{1}{m}\sum_{i=1}^{m}(\sigma(z^{(i)}) - y^{(i)})x_j^{(i)}$
2. $\frac{\partial J}{\partial w_j} = \frac{1}{m}\sum_{i=1}^{m}(\sigma(z^{(i)}) - y^{(i)})x_j^{(i)} + \frac{\lambda}{m}w_j$
3. $\frac{\partial J}{\partial w_j} = -\frac{1}{m}\sum_{i=1}^{m}[y^{(i)}(1-\sigma(z^{(i)})) - (1-y^{(i)})\sigma(z^{(i)})]x_j^{(i)}$
4. $\frac{\partial J}{\partial w_j} = -\frac{1}{m}\sum_{i=1}^{m}[y^{(i)}\log(\sigma(z^{(i)})) - (1-y^{(i)})\log(1-\sigma(z^{(i)}))]x_j^{(i)} + \frac{\lambda}{2m}w_j^2$
5. $\frac{\partial J}{\partial w_j} = \frac{1}{m}\sum_{i=1}^{m}(\sigma(z^{(i)}) - y^{(i)}) + \frac{\lambda}{2m}w_j^2$

## Solution
To find the gradient of the cost function $J(w)$ with respect to each weight $w_j$, we start by recognizing that the derivative of the sigmoid function $\sigma(z)$ with respect to $z$ is $\sigma(z)(1-\sigma(z))$, and the derivative of $z$ with respect to $w_j$ is $x_j^{(i)}$ for the $i$-th training example. 

We also acknowledge that the cost function $J(w)$ is composed of two terms: the loss term and the regularization term. The derivative is computed separately for each part and then summed. 

1. For the loss term, the derivative with respect to $w_j$ (where $j \ge 1$ to exclude the bias term from regularization) is obtained by applying the chain rule:

$$\frac{\partial J}{\partial w_j} = -\frac{1}{m}\sum_{i=1}^{m} [y^{(i)}\frac{\sigma(z^{(i)})(1-\sigma(z^{(i)}))}{\sigma(z^{(i)})} - (1-y^{(i)})\frac{\sigma(z^{(i)})(1-\sigma(z^{(i)}))}{1-\sigma(z^{(i)})}]x_j^{(i)}$$

This simplifies to:

$$\frac{\partial J}{\partial w_j} = \frac{1}{m}\sum_{i=1}^{m}(\sigma(z^{(i)}) - y^{(i)})x_j^{(i)}$$

2. For the regularization term, the derivative with respect to $w_j$ is:

$$\frac{\partial}{\partial w_j} \frac{\lambda}{2m}\sum_{j=1}^{n}w_j^2 = \frac{\lambda}{m}w_j$$ 

Adding the derivatives of the loss term and the regularization term gives the complete derivative:

$$\frac{\partial J}{\partial w_j} = \frac{1}{m}\sum_{i=1}^{m}(\sigma(z^{(i)}) - y^{(i)})x_j^{(i)} + \frac{\lambda}{m}w_j$$

Hence, the correct answer is that the derivative of the cost function with respect to $w_j$, incorporating the influence of the L2 regularization term, is:

$$\frac{\partial J}{\partial w_j} = \frac{1}{m}\sum_{i=1}^{m}(\sigma(z^{(i)}) - y^{(i)})x_j^{(i)} + \frac{\lambda}{m}w_j$$

## Correct Answer
2. $\frac{\partial J}{\partial w_j} = \frac{1}{m}\sum_{i=1}^{m}(\sigma(z^{(i)}) - y^{(i)})x_j^{(i)} + \frac{\lambda}{m}w_j$

## Reasoning
The reasoning boils down to two fundamental components: understanding the derivative of the sigmoid function within the binary cross-entropy loss formula and recognizing the impact of L2 regularization on the cost function. The sigmoid function's gradient is essential for computing the change in loss with respect to the model's weights during training, and the regularization term is crucial for controlling overfitting by penalizing large weights. The correct option systematically synthesizes these elements, reflecting not just the basic logistic regression mechanism but also an appreciation for the nuanced role of regularization in machine learning.